

Fusion Plasma Theory 2

Lecture 14: Hot Plasma Wave Dispersion.

① Perturbation during cyclotron motion in magnetized plasmas

- Kinetic effects in plasma waves: cyclotron harmonics and harmonic damping.
- Harmonics of cyclotron frequency = Finite-Larmor-Radius (FLR) effect.

$$\vec{E} = \hat{x} E_x e^{i(kx - \omega t)} \Rightarrow \ddot{x} + \omega_c^2 x = \frac{q}{m} E_x e^{i(kx - \omega t)}$$

- Method of characteristics: $x = r_L \sin(\omega_c t)$ + unperturbed orbit.

(무슨 일이 있든간에 particle의 위치는 이미 정해져있다고 생각하기)

$$\Rightarrow \ddot{x} + \omega_c^2 x = \frac{q}{m} E_x e^{i(kr_L \sin \omega_c t - \omega t)}$$

- Incredible identity:

$$e^{iz \sin \phi} = \sum_{n=-\infty}^{\infty} J_n(z) e^{in\phi} \quad \left(\Leftarrow e^{z(t - \frac{1}{t})/2} = \sum_{n=-\infty}^{\infty} J_n(z) t^n \text{ with } t = e^{i\phi} \right)$$

② Cyclotron harmonic resonances

$$z = kr_L, \phi = \omega_c t \Rightarrow \ddot{x} + \omega_c^2 x = \frac{q}{m} E_x \sum_{n=-\infty}^{\infty} J_n(kr_L) e^{-i(\omega - n\omega_c)t}$$

$$\text{let } x_n(t) = A_n e^{-i(\omega - n\omega_c)t}, \text{ then } [\omega_c^2 - (\omega - n\omega_c)^2] A_n = \frac{q}{m} E_x J_n(kr_L)$$

$$\Rightarrow A_n = \frac{\frac{q}{m} E_x J_n(kr_L)}{\omega_c^2 - (\omega - n\omega_c)^2} \Rightarrow x(t) = \frac{q}{m} E_x \sum_{n=-\infty}^{\infty} \frac{J_n(kr_L) e^{-i(\omega - n\omega_c)t}}{\omega_c^2 - (\omega - n\omega_c)^2}$$

- resonance occurs when $\omega = (n \pm 1)\omega_c$
- For small $kr_L \ll 1$, $J_n(kr_L) \sim \left(\frac{kr_L}{2}\right)^n / n!$ \rightarrow higher harmonics has weaker amplitude by $n!$
- when $kr_L \rightarrow 0$, $J_n(kr_L) \rightarrow 0$ ($n \neq 0$) \rightarrow For $n=0$, resonance only occurs $\omega = \pm \omega_c$ (fluid limit)
 $\quad \quad \quad \nearrow 1$ ($n=0$)
- Particle gains energy so the wave will lose energy \rightarrow cyclotron damping.
 It occurs always and does not require $df/dv < 0$ unlike Landau damping.

③ Vlasov equation for magnetized plasmas

Now consider kinetic waves through \vec{B}_0 . (Assume $f = f_0 + f_1$ and $\vec{E} = \vec{E}_1$)

$$\frac{df}{dt} + \vec{v} \cdot \frac{df}{d\vec{x}} + \frac{q}{m} (\vec{E} + \vec{v} \times \vec{B}) \frac{df}{d\vec{v}} = 0$$

\Downarrow

$$\frac{df_1}{dt} + \vec{v} \cdot \frac{df_1}{d\vec{x}} + \frac{q}{m} (\vec{v} \times \vec{B}_0) \frac{df_1}{d\vec{v}} + \frac{q}{m} (\vec{E}_1 + \vec{v} \times \vec{B}_1) \frac{df_0}{d\vec{v}} = 0$$

$$\Rightarrow \underbrace{\frac{Df_1}{Dt}}_{f_1} = \underbrace{\frac{df_1}{dt} + \vec{v} \cdot \frac{df_1}{d\vec{x}} + \frac{q}{m} (\vec{v} \times \vec{B}_0) \frac{df_1}{d\vec{v}}}_{f_1} = - \underbrace{\frac{q}{m} (\vec{E}_1 + \vec{v} \times \vec{B}_1) \frac{df_0}{d\vec{v}}}_{f_0}$$

Direct Fourier (or Laplace) approach X work due to $df_1/d\vec{v}$ which leads to non-linear equation.

Integrate the RHS along w/ unperturbed trajectory (\vec{x}', \vec{v}', t') when calculating \vec{E}_1 and \vec{B}_1

$$f_1(\vec{x}, \vec{v}, t) = - \frac{q}{m} \int_{-\infty}^t (\underbrace{\vec{E}_1(\vec{x}', t')}_{\text{background}} + \underbrace{\vec{v}' \times \vec{B}_1(\vec{x}', t')}_{\text{background}}) \frac{df_0(\vec{v}')}{d\vec{v}'} dt' \quad \left(\begin{array}{l} \star f_1 \text{을 구하려고 하지만,} \\ f_1 \text{이 움직이는 경로는 } f_0 \text{을 지배하는} \\ \text{background에 의해 결정된다} \end{array} \right)$$

Unperturbed trajectory (\vec{x}', \vec{v}') becomes (\vec{x}, \vec{v}) as $t' \rightarrow t$

The unperturbed trajectory in uniform plasma:

$$\frac{d\vec{x}}{dt} = \vec{v}, \quad \frac{d\vec{v}}{dt} = \frac{q}{m} \vec{v} \times \vec{B}_0$$

\star 입자의 궤적 자체는 B_0 에 의한 Helix with gyration만 한다.

④ Unperturbed particle trajectory

$$\vec{B}_0 = \hat{z} B_0, \quad \vec{v} = (v_{\perp} \cos \phi, v_{\perp} \sin \phi, v_{\parallel}) \rightarrow \vec{v}' = (v_{\perp} \cos(\omega_c \tau + \phi), v_{\perp} \sin(\omega_c \tau + \phi), v_{\parallel})$$

where $\tau \equiv t - t'$

Integrating in time:

$$\left(\begin{array}{l} x' - x = -\frac{v_{\perp}}{\omega_c} (\sin(\omega_c \tau + \phi) - \sin \phi) \\ y' - y = \frac{v_{\perp}}{\omega_c} (\cos(\omega_c \tau + \phi) - \cos \phi) \\ z' - z = -v_{\parallel} \tau \end{array} \right) \quad \star \tau=0 \text{ 이면 } x=x', y=y', z=z'$$

In our approach $f_0 = f_0(v_{\perp}, v_{\parallel})$ anisotropy with $v_{\perp} = (v_x'^2 + v_y'^2)^{1/2}$

$$\left(\begin{array}{l} \frac{df_0}{dv_x} = \frac{dv_{\perp}}{dv_x} \frac{df_0}{dv_{\perp}} = \frac{v_x'}{v_{\perp}} \frac{df_0}{dv_{\perp}} = \cos(\omega_c \tau + \phi) \frac{df_0}{dv_{\perp}} \\ \frac{df_0}{dv_y} = \frac{dv_{\perp}}{dv_y} \frac{df_0}{dv_{\perp}} = \frac{v_y'}{v_{\perp}} \frac{df_0}{dv_{\perp}} = \sin(\omega_c \tau + \phi) \frac{df_0}{dv_{\perp}} \\ \frac{df_0}{dv_z} = \frac{df_0}{dv_{\parallel}} \end{array} \right)$$

⑤ Perturbed distribution function by waves

Now consider perturbations $\sim e^{i(\vec{k} \cdot \vec{x} - \omega t)}$. Let $\vec{k} = k_\perp \hat{x} + k_\parallel \hat{z}$.

$$f_1 = -\frac{q}{m} \int_0^\infty \left[(E_x + \cancel{V_y' B_z} - \cancel{V_z' B_y}) \frac{df_0}{dV_x} + (E_y + \cancel{V_z' B_x} - \cancel{V_x' B_z}) \frac{df_0}{dV_y} + (E_z + V_x' B_y - V_y' B_x) \frac{df_0}{dV_z} \right] \cdot e^{i(\vec{k} \cdot (\vec{x}' - \vec{x}) - \omega(t' - t))} d\tau$$

$$= -\frac{q}{m} \int_0^\infty \left[(E_x - V_{\perp 1} B_y) \cos(\omega_c \tau + \phi) \frac{df_0}{dV_x} + (E_y + V_{\perp 1} B_x) \sin(\omega_c \tau + \phi) \frac{df_0}{dV_y} \right. \\ \left. + (E_z + V_{\perp 1} \cos(\omega_c \tau + \phi) B_y - V_{\perp 1} \sin(\omega_c \tau + \phi) B_x) \frac{df_0}{dV_z} \right] \times \exp \left[-i \frac{v_\perp}{\omega_c} (\sin(\omega_c \tau + \phi) - \sin \phi) + i(\omega - k_\parallel v_\parallel) \tau \right] d\tau$$

* note that $\frac{d\vec{B}_1}{dt} = -\vec{\nabla} \times \vec{E}_1 \rightarrow \omega \vec{B}_1 = \vec{k} \times \vec{E}_1 \Rightarrow B_x = -k_z E_y / \omega, B_y = (k_z E_x - k_x E_y) / \omega, B_z = k_x B_y / \omega$

Then, one can estimate j_1 for dielectric tensor ($\vec{j}_1 = \hat{\sigma} \cdot \vec{E}_1$)

$$\vec{j}_1 = q \int d\vec{v} (\hat{x} v_x \cos \phi + \hat{y} v_y \sin \phi + \hat{z} v_\parallel) f_1$$

⑥ Appendix - Bessel identities for kinetic integral. (결정 해야 하는 integral)

$$e^{iz \sin \phi} = \sum_{n=-\infty}^{\infty} J_n(z) e^{in\phi}$$

$$\int d\vec{v} = \int_0^{2\pi} d\phi \int dV_\perp \int dV_\parallel$$

알맞은 이커먼저하자

$$\int_0^{2\pi} d\phi e^{iz \sin \phi - iz \sin(\phi + \omega_c \tau)} = \int_0^{2\pi} d\phi \sum_n J_n e^{in\phi} \sum_m J_m e^{-im(\phi + \omega_c \tau)}$$

$$= 2\pi \sum_{n=-\infty}^{\infty} e^{-in\omega_c \tau} \begin{pmatrix} J_n J_n' \\ -i(n/z) J_n J_n' \\ i(n/z) J_n J_n' \\ (n^2/z^2) J_n J_n \\ J_n J_n \\ -i J_n J_n' \\ (n/z) J_n J_n \\ i J_n J_n' \\ (n/z) J_n J_n \end{pmatrix}$$

example) (i) $\int d\phi e^{iz \sin \phi - iz \sin(\phi + \omega_c \tau)} = \int d\phi \sum_n J_n e^{in\phi} \sum_m J_m e^{-im(\phi + \omega_c \tau)}$

$$= \begin{cases} 0 & (m \neq n) \\ 2\pi \sum_n J_n J_n e^{-in\omega_c \tau} & (m=n) \end{cases}$$

(ii) $\int d\phi e^{iz \sin \phi - iz \sin(\phi + \omega_c \tau)} \sin \phi \cos(\phi + \omega_c \tau)$

$$\left(\frac{d}{dz} (e^{iz \sin \phi} = \sum_n J_n e^{in\phi}) \rightarrow i \sin \phi e^{iz \sin \phi} = \sum_n J_n' e^{in\phi} \rightarrow \sin \phi e^{iz \sin \phi} = -i \sum_n J_n' e^{in\phi} \right.$$

$$\left. \frac{d}{d\phi} (e^{-iz \sin(\phi + \omega_c \tau)} = \sum_m J_m e^{-im(\phi + \omega_c \tau)}) \rightarrow -iz \cos(\phi + \omega_c \tau) e^{-iz \sin(\phi + \omega_c \tau)} = -i \sum_m m J_m e^{-im(\phi + \omega_c \tau)} \right)$$

$$= 2\pi \sum_n e^{-in\omega_c \tau} \left[-i \left(\frac{n}{z} \right) J_n J_n' \right]$$

Also, $\int_0^\infty \exp[i(\omega - k_{\parallel} v_{\parallel} - n\omega_c)z] dz = \frac{\exp(i(\dots)z)}{i(\omega - k_{\parallel} v_{\parallel} - n\omega_c)} \Big|_0^\infty = \frac{i}{\omega - k_{\parallel} v_{\parallel} - n\omega_c}$ provided $\text{Im}(\omega) > 0$
 0이 아니라 ∞ 에서 0이 됨

⑦ Kinetic dielectric tensor in magnetized plasmas

Then after performing dp and dz integral, we get:

$$\overleftrightarrow{\epsilon} = \overleftrightarrow{I} + \sum_S \frac{W_{PS}^2}{\omega^2} \sum_{n=-\infty}^{\infty} \int \frac{\overleftrightarrow{S}}{\omega - k_{\parallel} v_{\parallel} - n\omega_c} 2\pi d v_{\perp} d v_{\parallel}$$

where $\overleftrightarrow{S} = \begin{pmatrix} \frac{n^2 J_n^2}{Z^2} v_{\perp} U & i \frac{n J_n J_n'}{Z} v_{\perp} U & \frac{n J_n^2}{Z} v_{\perp} W \\ -i \frac{n J_n J_n'}{Z} v_{\perp} U & (J_n')^2 v_{\perp} U & -i J_n J_n' v_{\perp} W \\ \frac{n J_n^2}{Z} v_{\parallel} U & i J_n J_n' v_{\parallel} U & J_n^2 v_{\parallel} W \end{pmatrix}$ with $U \equiv (\omega - k_{\parallel} v_{\parallel}) \frac{df_{S0}}{dv_{\perp}} + k_{\parallel} v_{\perp} \frac{df_{S0}}{dv_{\parallel}}$
 $W \equiv \frac{n\omega_c \omega}{v_{\perp}} \frac{df_{S0}}{dv_{\perp}} + (\omega - n\omega_c) \frac{df_{S0}}{dv_{\parallel}}$

\overleftrightarrow{S} and \overleftrightarrow{S} is in a Hermitian form when the integral is performed. (Onsager symmetry)

⑧ Hot plasma dielectric tensor in magnetized Maxwellian

Identity: $\int_0^\infty t J_\nu(at) J_\nu(bt) e^{-p^2 t^2} dt = \frac{1}{2p^2} \exp\left(-\frac{a^2+b^2}{4p^2}\right) I_\nu\left(\frac{ab}{2p^2}\right)$

(I_ν = modified Bessel function of the first kind)

Kinetic dielectric tensor for Maxwellian plasmas:

$$\overleftrightarrow{\epsilon} = \overleftrightarrow{I} + \sum_S \frac{W_{PS}^2}{\omega^2} \sum_{\lambda_s} e^{-\lambda_s} \sum_{n=-\infty}^{\infty} \overleftrightarrow{T}$$

where $\overleftrightarrow{T} = \begin{pmatrix} \frac{n^2 I_n}{\lambda_s} Z & in(I_n' - I_n)Z & -\frac{n I_n}{(2\lambda_s)^{1/2}} Z' \\ -in(I_n' - I_n)Z & \left(\frac{n^2 I_n}{\lambda_s} + 2I_n \lambda_s - 2I_n' \lambda_s\right) Z & i \frac{(I_n' - I_n) \lambda_s^{1/2}}{2^{1/2}} Z' \\ -\frac{n I_n}{(2\lambda_s)^{1/2}} Z' & -i \frac{(I_n' - I_n) \lambda_s^{1/2}}{2^{1/2}} Z' & -I_n Z' \sum_{ns} \end{pmatrix}$

$\left(\begin{array}{l} I_n = I_n(\lambda_s), \quad \rightarrow \lambda_s \equiv \frac{k_{\perp}^2 v_{Ts}^2}{2n\omega_s^2} = \frac{1}{2} k_{\perp}^2 \rho_s^2 \ll 0 \\ Z = Z(\sum_{ns}) \quad \rightarrow \sum_{ns} = \frac{\omega - n\omega_{cs}}{k_{\parallel} v_{Ts}} \gg 0 \end{array} \right) \leftarrow \lambda \text{ dependency is FLR effect.}$

⑨ Hot plasma wave dispersion (Hot \rightarrow cold)

$$\epsilon_{ij} = \delta_{ij} + \sum_s \frac{W_{ps}^2}{W^2} \rho_{os} e^{-\lambda_s} \sum_{n=-\infty}^{\infty} T_{ij}$$

Assume $V_{Ts} \rightarrow 0 : \lambda_s \rightarrow 0$ and $\rho_{os} \rightarrow \infty$
 $\therefore I_n(\lambda_s) = \left(\frac{\lambda_s}{2}\right)^n, \quad Z(\rho_{os}) = -\frac{1}{\rho_{os}}$

(1) ϵ_{xx}

$$T_{xx} = \frac{n^2 I_n}{\lambda_s} Z(\rho_{os}) \rightarrow n^2 \frac{1}{\lambda_s} \left(\frac{\lambda_s}{2}\right)^n Z(\rho_{os}) = \begin{cases} 0 & (n=0) \\ \frac{1}{2} Z(\rho_{\pm 1s}) & (n=\pm 1) \\ 0 & (|n| \geq 2) \end{cases}$$

*note $I_n = I_{-n}$
 so it's defined
 only for $n \geq 0$

$$\sum_{n=-\infty}^{\infty} T_{xx} = \frac{1}{2} Z(\rho_{1s}) + \frac{1}{2} Z(\rho_{-1s}) = -\frac{1}{2} \frac{1}{\rho_{1s}} - \frac{1}{2} \frac{1}{\rho_{-1s}}$$

$$\left(\rho_{\pm 1s} = \frac{W \mp W_{cs}}{k_{\parallel} V_{Ts}}, \quad \rho_{os} = \frac{W}{k_{\parallel} V_{Ts}} \right)$$

$$\rho_{os} \sum_{n=-\infty}^{\infty} T_{xx} = \frac{W}{k_{\parallel} V_{Ts}} \frac{1}{2} \left[-\frac{k_{\parallel} V_{Ts}}{W - W_{cs}} - \frac{k_{\parallel} V_{Ts}}{W + W_{cs}} \right] = -\frac{W}{2} \left(\frac{1}{W - W_{cs}} + \frac{1}{W + W_{cs}} \right) = -\frac{W}{2} \frac{2W}{W^2 - W_{cs}^2}$$

$$= -\frac{W^2}{W^2 - W_{cs}^2}$$

$$\therefore \epsilon_{xx} = 1 + \sum_s \frac{W_{ps}^2}{W^2} \left(-\frac{W^2}{W^2 - W_{cs}^2} \right) = 1 - \sum_s \frac{W_{ps}^2}{W^2 - W_{cs}^2} = S \quad \text{where } S = 1 - \sum_s \frac{W_{ps}^2}{W^2 - W_{cs}^2}$$

(2) $\epsilon_{xy} = -\epsilon_{yx}$

$$T_{xy} = -in(I_n' - I_n) \rightarrow -in \left(\frac{n}{2} \left(\frac{\lambda_s}{2}\right)^{n-1} - \left(\frac{\lambda_s}{2}\right)^n \right) Z(\rho_{os}) = \begin{cases} 0 & (n=0) \\ \mp i \frac{1}{2} Z(\rho_{ns}) & (n=\pm 1) \\ 0 & (|n| \geq 2) \end{cases}$$

$$\sum_{n=-\infty}^{\infty} T_{xy} = -\frac{i}{2} Z(\rho_{1s}) + \frac{i}{2} Z(\rho_{-1s}) = +\frac{i}{2} \left(\frac{1}{\rho_{1s}} - \frac{1}{\rho_{-1s}} \right)$$

$$\rho_{os} \sum_{n=-\infty}^{\infty} T_{xy} = \frac{W}{k_{\parallel} V_{Ts}} \frac{-i}{2} \left(\frac{k_{\parallel} V_{Ts}}{W + W_{cs}} - \frac{k_{\parallel} V_{Ts}}{W - W_{cs}} \right) = \frac{-Wi}{2} \frac{-2W_{cs}}{W^2 - W_{cs}^2} = +i \frac{W W_{cs}}{W^2 - W_{cs}^2}$$

$$\therefore \epsilon_{xy} = \sum_s \frac{W_{ps}^2}{W^2} \left(+i \frac{W W_{cs}}{W^2 - W_{cs}^2} \right) = +i \sum_s \frac{W_{cs}}{W} \frac{W_{ps}^2}{W^2 - W_{cs}^2} = +iD \quad \text{where } D = \sum_s \frac{W_{cs}}{W} \frac{W_{ps}^2}{W^2 - W_{cs}^2}$$

(3) ϵ_{zz}

$$T_{zz} = -I_n Z' \rho_{ns} \rightarrow -\left(\frac{\lambda_s}{2}\right)^n Z' \rho_{ns} = \begin{cases} -Z' \rho_{0s} & (n=0) \\ 0 & (|n| \geq 1) \end{cases}$$

$$\sum_{n=-\infty}^{\infty} T_{zz} = -Z' \rho_{0s} = \frac{-1}{\rho_{0s}^2} \rho_{0s} = -\frac{1}{\rho_{0s}}$$

$$\rho_{0s} \sum_{n=-\infty}^{\infty} T_{zz} = \rho_{0s} \left(-\frac{1}{\rho_{0s}}\right) = -1$$

$$\therefore \epsilon_{zz} = 1 + \sum \frac{w_{ps}^2}{\omega^2} (-1) = 1 - \sum \frac{w_{ps}^2}{\omega^2} = \rho \quad \text{where } \rho = 1 - \sum \frac{w_{ps}^2}{\omega^2}$$

(4) $\epsilon_{xz} = \epsilon_{zx}$

$$T_{xz} = -\frac{n I_n}{(2\lambda_s)^{1/2}} Z' \rightarrow -\frac{n \left(\frac{\lambda_s}{2}\right)^n}{(2\lambda_s)^{1/2}} Z' \sim \begin{cases} 0 & (n=0) \\ \sqrt{\lambda} Z' & (n=1) \sim \sqrt{\lambda} \left(\frac{1}{\rho_{0s}^2}\right) \rightarrow 0 \\ \lambda^{3/2} Z' & (n=2) \sim \sqrt{\lambda} \left(\frac{1}{\rho_{0s}^2}\right) \rightarrow 0 \end{cases}$$

$$\therefore \epsilon_{xz} = \sum \frac{w_{ps}^2}{\omega^2} \cdot 0 = 0$$

(5) $\epsilon_{yz} = \epsilon_{zy}$

$$T_{yz} = -i \frac{(I_n' - I_n) \lambda_s^{1/2}}{2^{1/2}} Z' \rightarrow -i \frac{\left(\frac{n}{2} \left(\frac{\lambda_s}{2}\right)^{n-1} - \left(\frac{\lambda_s}{2}\right)^n\right) \lambda_s^{1/2}}{2^{1/2}} Z' \sim \begin{cases} -i \left(\frac{\lambda_s}{2}\right)^{1/2} & (n=0) \rightarrow 0 \\ -i \left(\frac{\lambda_s}{8}\right)^{1/2} & (n=1) \rightarrow 0 \\ \vdots \end{cases}$$

$$\therefore \epsilon_{yz} = \epsilon_{zy} \approx 0$$

(6) ϵ_{yy}

$$T_{yy} = \left(\frac{n^2 I_n}{\lambda_s} + 2I_n \lambda_s - 2I_n' \lambda_s\right) Z \rightarrow \left(\frac{n^2}{\lambda_s} \left(\frac{\lambda_s}{2}\right)^n + 2\left(\frac{\lambda_s}{2}\right)^n \lambda_s - n \left(\frac{\lambda_s}{2}\right)^{n-1} \lambda_s\right) Z$$

$$= \begin{cases} 0 & (n=0) \\ \frac{1}{2} Z(\rho_{ns}) & (n=\pm 1) \\ 0 & (|n| \geq 2) \end{cases}$$

$$\Rightarrow \sum_{n=-\infty}^{\infty} T_{yy} = \frac{1}{2} Z(\rho_{1s}) + \frac{1}{2} Z(\rho_{-1s}) = -\frac{1}{2} \frac{1}{\rho_{1s}} - \frac{1}{2} \frac{1}{\rho_{-1s}}$$

$$\rho_{0s} \sum_{n=-\infty}^{\infty} T_{yy} = \frac{w}{k_{\perp} w_{Ts}} \frac{1}{2} \left[-\frac{k_{\perp} w_{Ts}}{w - w_{cs}} - \frac{k_{\perp} w_{Ts}}{w + w_{cs}} \right] = -\frac{w}{2} \frac{2w}{w^2 - w_{cs}^2} = -\frac{w^2}{w^2 - w_{cs}^2}$$

$$\therefore \epsilon_{yy} = 1 + \sum \frac{w_{ps}^2}{\omega^2} \left(-\frac{w^2}{w^2 - w_{cs}^2} \right) = 1 - \sum \frac{w_{pi}^2}{\omega^2 - w_{cs}^2} = S$$

In cold plasma limit,

$$\vec{\epsilon} \approx \begin{pmatrix} S & -iD & 0 \\ iD & S & 0 \\ 0 & 0 & P \end{pmatrix}$$

⑩ Hot parallel wave dispersion $\star (k_{\perp} \rightarrow 0, \lambda_s \rightarrow 0)$ $O(\lambda_s)$ for \vec{T} becomes

$$\vec{T} = \begin{pmatrix} (Z_{is} + Z_{-is})/2 & i(Z_{is} - Z_{-is})/2 & 0 \\ -i(Z_{is} - Z_{-is})/2 & (Z_{is} + Z_{-is})/2 & 0 \\ 0 & 0 & -Z'_{os} \rho_{os} \end{pmatrix}$$

* Recall

$$\vec{\epsilon} = \vec{I} + \sum_s \frac{\omega_{ps}^2}{\omega^2} \rho_{os} e^{-\lambda_s} \vec{T} \quad \text{and} \quad S = \frac{R+L}{2}, \quad D = \frac{R-L}{2}$$

$$\left\{ \begin{array}{l} S = \epsilon_{xx} = \epsilon_{yy} = 1 + \sum_s \frac{\omega_{ps}^2}{\omega^2} \rho_{os} \frac{Z_{is} + Z_{-is}}{2} \\ D = -\epsilon_{xy} = \epsilon_{yx} = \sum_s \frac{\omega_{ps}^2}{\omega^2} \rho_{os} \left(\frac{-Z_{is} + Z_{-is}}{2} \right) \\ P = \epsilon_{zz} = 1 - \sum_s \frac{\omega_{ps}^2}{\omega^2} \rho_{os}^2 Z'(\rho_{os}) \end{array} \right\} \Rightarrow \left\{ \begin{array}{l} R = 1 + \sum_s \frac{\omega_{ps}^2}{\omega^2} \rho_{os} Z_{-is} \\ L = 1 + \sum_s \frac{\omega_{ps}^2}{\omega^2} \rho_{os} Z_{is} \\ P = 1 - \sum_s \frac{\omega_{ps}^2}{\omega^2} \rho_{os}^2 Z'(\rho_{os}) \end{array} \right\}$$

⑪ Cyclotron damping of parallel wave

Hot plasma oscillation $P=0 \rightarrow 1 = \sum_s \frac{\omega_{ps}^2}{\omega^2} \frac{\omega^2}{k_{\parallel} v_{ts}} Z'(\rho_{os}) \rightarrow k_{\parallel}^2 = \sum_s \frac{\omega_{ps}^2}{v_{ts}^2} Z'(\rho_{os})$

R-wave $n_{\parallel}^2 = R \rightarrow n_{\parallel}^2 = 1 + \sum_s \frac{\omega_{ps}^2}{\omega k_{\parallel} v_{ts}} Z\left(\frac{\omega + \omega_{cs}}{k_{\parallel} v_{ts}}\right)$

L-wave $n_{\parallel}^2 = L \rightarrow n_{\parallel}^2 = 1 + \sum_s \frac{\omega_{ps}^2}{\omega k_{\parallel} v_{ts}} Z\left(\frac{\omega - \omega_{cs}}{k_{\parallel} v_{ts}}\right)$

\Rightarrow condition for ^{significant} R, L wave damping

R wave : $\omega - \omega_{ce} \leq k_{\parallel} v_{te}$

L wave : $\omega + \omega_{ce} \leq k_{\parallel} v_{ti}$

⑪ Hot perpendicular wave dispersion ($k_{||} \rightarrow 0$, $S_{ns} \rightarrow \infty$, $Z \rightarrow -(\frac{1}{S_{ns}})$)

$$\begin{pmatrix} \epsilon_{xx} & \epsilon_{xy} & 0 \\ -\epsilon_{xy} & \epsilon_{yy} - n_{\perp}^2 & 0 \\ 0 & 0 & \epsilon_{zz} - n_{\perp}^2 \end{pmatrix} \begin{pmatrix} E_x \\ E_y \\ E_z \end{pmatrix} = 0$$

$$T_{zz} = -I_n Z' S_{ns} = -I_n \frac{1}{S_{ns}} = -I_n \frac{k_{||} v_{ts}}{\omega - n\omega_{cs}}$$

$$\epsilon_{zz} = 1 + \sum_s \frac{W_{ps}^2}{W^2} S_{os} e^{-\lambda_s} \sum_{n=-\infty}^{\infty} T_{zz} = 1 - \sum_s \frac{W_{ps}^2}{W} e^{-\lambda_s} \sum_{n=-\infty}^{\infty} \frac{I_n(\lambda_s)}{W - n\omega_{cs}}$$

$$\therefore \text{O-wave } (n_{\perp}^2 = P) \rightarrow \left(n_{\perp}^2 = 1 - \sum_s \frac{W_{ps}^2}{W} e^{-\lambda_s} \sum_{n=-\infty}^{\infty} \frac{I_n(\lambda_s)}{W - n\omega_{cs}} \right)$$

$$\text{X-wave } (n_{\perp}^2 = \frac{RL}{S} = \epsilon_{yy} + \frac{\epsilon_{xy}^2}{\epsilon_{xx}})$$

$$\rightarrow \left(n_{\perp}^2 = 1 - \sum_s \frac{W_{ps}^2}{W} \frac{e^{-\lambda_s}}{\lambda_s} \sum_{n=-\infty}^{\infty} \frac{n^2 I_n(\lambda_s) + 2\lambda_s^2 I_n(\lambda_s) - 2\lambda_s^2 I_n'(\lambda_s)}{W - n\omega_{cs}} \right. \\ \left. - \frac{\left[\sum_s \frac{W_{ps}^2}{W} e^{-\lambda_s} \sum_{n=-\infty}^{\infty} \frac{n(I_n' - I_n)}{W - n\omega_{cs}} \right]^2}{1 - \sum_s \frac{W_{ps}^2}{W} \frac{e^{-\lambda_s}}{\lambda_s} \sum_{n=-\infty}^{\infty} \frac{n^2 I_n}{W - n\omega_{cs}}} \right)$$

⑫ Cyclotron harmonic damping

In either O or X-wave, one can see new class of resonance due to cyclotron harmonic frequency $\omega \approx n\omega_c$. These resonances are FLR effects.

$$\frac{1}{\omega - kv_{||} - n\omega_{cs}} \rightarrow P \left(\frac{1}{\omega - kv_{||} - n\omega_{cs}} \right) - i\pi \delta(\omega - kv_{||} - n\omega_{cs})$$

There is another class of solution with small wavelength $n_{\perp} = k_{\perp} c / \omega \gg 1$

$$\epsilon_{xx} = 0 = 1 - \sum_s \frac{W_{ps}^2}{W} \frac{e^{-\lambda_s}}{\lambda_s} \sum_{n=-\infty}^{\infty} \frac{n^2 I_n(\lambda_s)}{W - n\omega_{cs}} \quad : \text{Bernstein wave}$$